lean4/Automaton/Regex/Basic.lean
@@ -1,0 +1,71 @@
+import Automaton.Language.Basic
+import Mathlib.Data.Finset.Basic
+import Mathlib.Data.Fin.Basic
+import Automaton.NFA.ENFA
+
+namespace Regex
+
+open Set Finset εNFA
+
+inductive Regex (f : Finset α) : Type u
+  | zero : Regex f
+  | epsilon : Regex f
+  | char : (α : f) → Regex f
+  | plus : Regex f → Regex f → Regex f
+  | append : Regex f → Regex f → Regex f
+  | star : Regex f → Regex f
+
+open Regex
+
+variable {α : Type _} [DecidableEq α] (f : Finset α)
+
+inductive starLang (l : Lang f) : Lang f where
+  | empty : starLang l []
+  | star  : ∀ u w : List f, u ∈ l → w ∈ l → starLang l (u++w)
+
+def RegexLan : Regex f → Lang f
+  | zero => ∅
+  | epsilon => {[]}
+  | char a => {[a]}
+  | plus a b => RegexLan a ∪ RegexLan b
+  | append a b => {w | ∃ x y, x ∈ RegexLan a ∧ y ∈ RegexLan b ∧ w = x++y}
+  | star a => starLang f (RegexLan a)
+
+
+def ZeroεNFA : εNFA f {0} := {q₀ := {⟨0,by simp⟩} , fs := {} , δ := fun _ _ => {⟨0,by simp⟩}}
+def EpsilonεNFA : εNFA f {0} := {q₀ := {⟨0,by simp⟩} , fs := {⟨0,by simp⟩} , δ := fun _ _ => ∅}
+def CharεNFA (c : f) : εNFA f {0,1} := {q₀ := {⟨0,by simp⟩} , fs := {⟨1,by simp⟩} , δ := fun q e => if q = ⟨0,by simp⟩ ∧ e = c then {⟨1,by simp⟩} else ∅}
+
+
+lemma ZeroεNFALang : εNFA_lang (ZeroεNFA f) = ∅ := by
+  simp only [εNFA_lang,εnfa_accepts,ZeroεNFA,Finset.inter_empty]
+  trivial
+
+
+lemma EpsilonεNFALang : εnfa_accepts (EpsilonεNFA f) w ↔ w = [] := by
+  apply Iff.intro
+  · intro ac
+    simp only [εnfa_accepts,EpsilonεNFA] at ac
+    match w with
+    | [] => simp
+    | e::es => simp only [δ_star,δ_star',Finset.Nonempty] at ac
+               apply Exists.elim ac
+               intro w win
+               simp [δ_step,Finset.biUnion] at win
+               rw [εNFA_δ_star'_empty] at win
+               simp
+               apply Finset.not_mem_empty
+               exact win.1
+  · intro w
+    rw [w]
+    simp [εnfa_accepts,δ_star,δ_star',EpsilonεNFA,Finset.Nonempty]
+    apply εclosure_start_mem
+    simp
+
+
+
+
+
+
+
+end Regex
